Lots of WIP
- Fix induction principle case for tv.
- Add variant of induction principle that allows predicate to depend on number
- of free vars (probably should replace the original).
- Fix vstampP for is_stamped.
- Lots of theorems.

theories/DSub/stampedness.v
@@ -31,7 +31,7 @@ Definition is_stamped_trav: Traversal (nat * stys) :=
     upS := λ '(n, g), (S n, g);
     varP := λ '(n, g) i, i < n;
     vtyP := λ ts T, False;
-    vstampP := λ '(n, g) vs s, length vs = n ∧ ∃ T, g !! s = Some T ∧ nclosed T n;
+    vstampP := λ '(n, g) vs s, ∃ T', g !! s = Some T' ∧ nclosed T' (length vs) ∧ nclosed_σ vs n;
   |}.
 
 Section fold.
@@ -92,15 +92,15 @@ Global Arguments varP /.
 Global Arguments vtyP /.
 Global Arguments vstampP /.
 
-Lemma stamped_idsσ_ren g m n j: j + n <= m → Forall (is_stamped_vl m g) (idsσ n).|[ren (+j)].
+Lemma is_stamped_idsσ_ren g m n j: j + n <= m → Forall (is_stamped_vl m g) (idsσ n).|[ren (+j)].
 Proof.
   elim: n m j => [|n IHn] m j Ijm //=.
   repeat constructor => //=; first lia.
   asimpl; apply IHn; lia.
 Qed.
 
-Lemma stamped_idsσ g m n: n <= m → Forall (is_stamped_vl m g) (idsσ n).
-Proof. pose proof (@stamped_idsσ_ren g m n 0) as H. asimpl in H. exact: H. Qed.
+Lemma is_stamped_idsσ g m n: n <= m → Forall (is_stamped_vl m g) (idsσ n).
+Proof. pose proof (@is_stamped_idsσ_ren g m n 0) as H. asimpl in H. exact: H. Qed.
 
 Hint Constructors forall_traversal_vl forall_traversal_ty forall_traversal_tm.
 
@@ -163,3 +163,245 @@ Lemma is_stamped_mono_ty g1 g2 n T__s:
   is_stamped_ty n g1 T__s →
   is_stamped_ty n g2 T__s.
 Proof. unmut_lemma is_stamped_mono_mut. Qed.
+
+Definition is_stamped_sub n m g s :=
+  ∀ i, i < n → is_stamped_vl m g (s i).
+Definition is_stamped_ren n m g r := is_stamped_sub n m g (ren r).
+
+Lemma is_stamped_ren_shift n m j g:
+  m >= j + n → is_stamped_ren n m g (+j).
+Proof. constructor => //=; lia. Qed.
+
+Lemma is_stamped_ren_up n m g r:
+  is_stamped_ren n m g r →
+  is_stamped_ren (S n) (S m) g (upren r).
+Proof.
+  (* rewrite /is_stamped_ren /is_stamped_sub /=. *)
+  move => Hr [|i] //= Hi; first by constructor => /=; lia.
+  have Hi': i < n by lia.
+  specialize (Hr i Hi'); inverse Hr.
+  constructor; cbn in *; by lia.
+Qed.
+Hint Resolve is_stamped_ren_up is_stamped_ren_shift.
+
+From D.DSub Require Import closed_subst.
+
+Lemma is_stamped_nclosed_ren i j g r: is_stamped_ren i j g r → nclosed_ren i j r.
+Proof.
+  move => /= Hr x Hx. specialize (Hr x Hx); inverse Hr. exact: nclosed_vl_ids.
+Qed.
+
+Lemma is_stamped_ren_mut:
+  (∀ t g r i j,
+    is_stamped_ren i j g r →
+    is_stamped_tm i g t →
+    is_stamped_tm j g (rename r t)) ∧
+  (∀ v g r i j,
+    is_stamped_ren i j g r →
+    is_stamped_vl i g v →
+    is_stamped_vl j g (rename r v)) ∧
+  (∀ T g r i j,
+    is_stamped_ren i j g r →
+    is_stamped_ty i g T →
+    is_stamped_ty j g (rename r T)).
+Proof.
+  apply syntax_mut_ind; intros; with_is_stamped ltac:(fun H => inversion_clear H);
+    cbn in *; try by [constructor; cbn; eauto].
+  - eauto.
+  - constructor. rewrite /= /rename /list_rename map_length /=.
+    ev; eexists; split_and!; eauto; rewrite Forall_fmap.
+    decompose_Forall.
+    eapply nclosed_ren_vl => //.
+    by eapply is_stamped_nclosed_ren.
+Qed.
+
+Lemma is_stamped_ren_vl: ∀ v g r i j,
+  is_stamped_ren i j g r →
+  is_stamped_vl i g v →
+  is_stamped_vl j g (rename r v).
+Proof. unmut_lemma is_stamped_ren_mut. Qed.
+
+Lemma is_stamped_sub_up n m g s:
+  is_stamped_sub n m g s →
+  is_stamped_sub (S n) (S m) g (up s).
+Proof.
+  move => Hs [|i] Hi //=. by constructor => /=; lia.
+  eapply is_stamped_ren_vl; eauto with lia.
+Qed.
+Hint Resolve is_stamped_sub_up.
+
+Lemma is_stamped_nclosed_mut g:
+  (∀ t i,
+    is_stamped_tm i g t →
+    nclosed t i) ∧
+  (∀ v i,
+    is_stamped_vl i g v →
+    nclosed_vl v i) ∧
+  (∀ T i,
+    is_stamped_ty i g T →
+    nclosed T i).
+Proof.
+  apply syntax_mut_ind; intros; with_is_stamped inverse => //;
+    cbn in *; ev; eauto using fv_vstamp;
+    move => s1 s2 Hseq /=; f_equal.
+  (* all: time try firstorder eauto using eq_up. (* 1.7 s *) *)
+  (* all: time try naive_solver; eauto using eq_up. (* 0.8s *) *)
+  all: try eapply H; eauto using eq_up.
+  all: try eapply H0; eauto using eq_up.
+Qed.
+
+Lemma is_stamped_nclosed_vl v g i:
+  is_stamped_vl i g v →
+  nclosed_vl v i.
+Proof. unmut_lemma (is_stamped_nclosed_mut g). Qed.
+
+Lemma is_stamped_nclosed_sub i j g s: is_stamped_sub i j g s → nclosed_sub i j s.
+Proof.
+  move => /= Hs x Hx. eapply is_stamped_nclosed_vl, (Hs x Hx).
+Qed.
+
+Lemma is_stamped_sub_mut:
+  (∀ t g s i j,
+    is_stamped_sub i j g s →
+    is_stamped_tm i g t →
+    is_stamped_tm j g t.|[s]) ∧
+  (∀ v g s i j,
+    is_stamped_sub i j g s →
+    is_stamped_vl i g v →
+    is_stamped_vl j g v.[s]) ∧
+  (∀ T g s i j,
+    is_stamped_sub i j g s →
+    is_stamped_ty i g T →
+    is_stamped_ty j g T.|[s]).
+Proof.
+  apply syntax_mut_ind; intros; with_is_stamped ltac:(fun H => inversion_clear H);
+    cbn in *; try by [constructor; cbn; eauto].
+  - eauto.
+  - constructor. rewrite /= map_length.
+    ev; eexists; split_and!; eauto; rewrite Forall_fmap.
+    decompose_Forall.
+    eapply nclosed_sub_vl => //.
+    exact: is_stamped_nclosed_sub.
+Qed.
+
+Lemma is_stamped_sub_vl v g s m n:
+  is_stamped_sub n m g s →
+  is_stamped_vl n g v →
+  is_stamped_vl m g v.[s].
+Proof. unmut_lemma is_stamped_sub_mut. Qed.
+
+Lemma is_stamped_sub_ty T g s m n:
+  is_stamped_sub n m g s →
+  is_stamped_ty n g T →
+  is_stamped_ty m g T.|[s].
+Proof. unmut_lemma is_stamped_sub_mut. Qed.
+
+Lemma is_stamped_sub_rev_vl g: ∀ v s i j,
+  nclosed_vl v i →
+  is_stamped_sub i j g s →
+  is_stamped_vl j g (v.[s]) →
+  is_stamped_vl i g v.
+Proof.
+  induction v; intros; constructor => //=; eauto;
+  with_is_stamped inverse; cbn in *; ev.
+  admit. done. done.
+  rewrite map_length in H3.
+  eexists; split_and!; eauto.
+  move: H4; rewrite /hsubst /list_hsubst Forall_fmap; move => Hcll.
+  decompose_Forall.
+Admitted.
+
+Lemma is_stamped_sub_rev_mut g:
+  (∀ e i,
+    nclosed e i →
+    ∀ s j, is_stamped_sub i j g s →
+    is_stamped_tm j g (e.|[s]) →
+    is_stamped_tm i g e) ∧
+  (∀ v i,
+    nclosed_vl v i →
+    ∀ s j, is_stamped_sub i j g s →
+    is_stamped_vl j g (v.[s]) →
+    is_stamped_vl i g v) ∧
+  (∀ T i,
+    nclosed T i →
+    ∀ s j, is_stamped_sub i j g s →
+    is_stamped_ty j g (T.|[s]) →
+    is_stamped_ty i g T).
+Proof.
+  apply nclosed_syntax_mut_ind => /=; intros;
+    try by with_is_stamped inverse; ev;
+    constructor => /=; eauto using eq_up with lia.
+  with_is_stamped inverse; cbn in *; ev.
+  constructor => /=.
+
+  rewrite map_length in H5.
+  eexists; split_and!; eauto.
+  move: H6; rewrite /hsubst /list_hsubst Forall_fmap; move => Hcll.
+  decompose_Forall.
+  specialize (H8 s0 j H2).
+
+  Lemma foo v i j s:
+  nclosed_vl v.[s] j →
+  nclosed_vl v i.
+  Admitted.
+  Admitted.
+
+(*
+Lemma is_stamped_sub_rev_mut g:
+  (∀ t s m n,
+    is_stamped_sub n m g s →
+    is_stamped_tm m g (t.|[s]) →
+    is_stamped_tm n g t) ∧
+  (∀ v s m n,
+    is_stamped_sub n m g s →
+    is_stamped_vl m g (v.[s]) →
+    is_stamped_vl n g v) ∧
+  (∀ T s m n,
+    is_stamped_sub n m g s →
+    is_stamped_ty m g (T.|[s]) →
+    is_stamped_ty n g T).
+Proof.
+  apply syntax_mut_ind => /=; intros;
+    try by with_is_stamped inverse; ev;
+    constructor => /=; eauto using eq_up with lia.
+  constructor => /=. *)
+
+(* Lemma is_stamped_sub_rev_mut g:
+  (∀ t s m n,
+    is_stamped_sub n m g s →
+    is_stamped_tm m g (t.|[s]) →
+    is_stamped_tm n g t) ∧
+  (∀ v s m n,
+    is_stamped_sub n m g s →
+    is_stamped_vl m g (v.[s]) →
+    is_stamped_vl n g v) ∧
+  (∀ T s m n,
+    is_stamped_sub n m g s →
+    is_stamped_ty m g (T.|[s]) →
+    is_stamped_ty n g T).
+Proof.
+  apply syntax_mut_ind => /=; intros;
+    try by with_is_stamped inverse; ev;
+    constructor => /=; eauto using eq_up with lia.
+  constructor => /=. *)
+  (* That's false! *)
+
+
+Lemma is_stamped_sub_rev_ty g T s m n:
+  is_stamped_sub n m g s →
+  is_stamped_ty m g (T.|[s]) →
+  is_stamped_ty n g T.
+Proof.
+  elim: T m n s => /=; intros; with_is_stamped inverse;
+    constructor => /=; eauto using eq_up.
+
+
+Admitted.
+
+Lemma is_stamped_ren_ty n T g:
+  is_stamped_ty n g T <->
+  is_stamped_ty (S n) g (T.|[ren (+1)]).
+Proof.
+  have Hs: is_stamped_sub n (S n) g (ren (+1)). by apply is_stamped_ren_shift; lia.
+  split; intros; by [ eapply is_stamped_sub_ty | eapply is_stamped_sub_rev_ty].
+Qed.
